engine/PrisonersDilemma.lean
@@ -7,8 +7,6 @@ import PrisonersDilemma.Models.Bots.CooperateBot
 import PrisonersDilemma.Models.Bots.DefectBot
 import PrisonersDilemma.Models.BotUniverse
 import PrisonersDilemma.Models.Bots.DBot
-import PrisonersDilemma.Models.OpenSourceBots
 import PrisonersDilemma.Proofs.CooperateBot
 import PrisonersDilemma.Proofs.DefectBot
 import PrisonersDilemma.Proofs.DBot
-import PrisonersDilemma.Proofs.OpenSourceBots
